pipit/plugin-test/bug-reproductions/Plugin.Test.Bug.MasterModes.V2b.SpliceLike.fst
@@ -1,0 +1,222 @@
+module Plugin.Test.Bug.MasterModes.V2b.SpliceLike
+
+module PXB = Pipit.Exp.Base
+module PPS = Pipit.Prim.Shallow
+module PPT = Pipit.Prim.Table
+module PSHS = Pipit.Prim.HasStream
+
+open Plugin.Test.Bug.MasterModes.Types
+open FStar.Pervasives.Native
+
+#set-options "--warn_error -242"
+
+unfold let __xprim_mm_v2b_opt_eq_int_46 : Pipit.Prim.Shallow.prim =
+  Pipit.Prim.Shallow.Mkprim (Some "Prims.op_Equality")
+  (Pipit.Prim.Table.FTFun (Pipit.Prim.HasStream.shallow (option master_index_int))
+      (Pipit.Prim.Table.FTFun (Pipit.Prim.HasStream.shallow (option master_index_int))
+          (Pipit.Prim.Table.FTVal (Pipit.Prim.HasStream.shallow bool))))
+  op_Equality
+
+unfold let __xprim_mm_v2b_opt_eq_int_45 : Pipit.Prim.Shallow.prim =
+  Pipit.Prim.Shallow.Mkprim (Some "Prims.op_disEquality")
+  (Pipit.Prim.Table.FTFun (Pipit.Prim.HasStream.shallow error_severity)
+      (Pipit.Prim.Table.FTFun (Pipit.Prim.HasStream.shallow error_severity)
+          (Pipit.Prim.Table.FTVal (Pipit.Prim.HasStream.shallow bool))))
+  op_disEquality
+
+unfold let __xprim_mm_v2b_opt_eq_int_44 : Pipit.Prim.Shallow.prim =
+  Pipit.Prim.Shallow.Mkprim (Some "FStar.Pervasives.Native.uu___is_Some")
+  (Pipit.Prim.Table.FTFun (Pipit.Prim.HasStream.shallow (option master_index_int))
+      (Pipit.Prim.Table.FTVal (Pipit.Prim.HasStream.shallow bool)))
+  Some?
+
+unfold let __xprim_mm_v2b_opt_eq_int_43 : Pipit.Prim.Shallow.prim =
+  Pipit.Prim.Shallow.Mkprim (Some "Prims.op_AmpAmp")
+  (Pipit.Prim.Table.FTFun (Pipit.Prim.HasStream.shallow bool)
+      (Pipit.Prim.Table.FTFun (Pipit.Prim.HasStream.shallow bool)
+          (Pipit.Prim.Table.FTVal (Pipit.Prim.HasStream.shallow bool))))
+  op_AmpAmp
+
+unfold let __xprim_mm_v2b_opt_eq_int_42 : Pipit.Prim.Shallow.prim =
+  Pipit.Prim.Shallow.Mkprim (Some "Prims.op_Equality")
+  (Pipit.Prim.Table.FTFun (Pipit.Prim.HasStream.shallow master_mode)
+      (Pipit.Prim.Table.FTFun (Pipit.Prim.HasStream.shallow master_mode)
+          (Pipit.Prim.Table.FTVal (Pipit.Prim.HasStream.shallow bool))))
+  op_Equality
+
+unfold let __xprim_mm_v2b_opt_eq_int_41 : Pipit.Prim.Shallow.prim =
+  Pipit.Prim.Shallow.Mkprim (Some "Prims.op_Equality")
+  (Pipit.Prim.Table.FTFun (Pipit.Prim.HasStream.shallow error_severity)
+      (Pipit.Prim.Table.FTFun (Pipit.Prim.HasStream.shallow error_severity)
+          (Pipit.Prim.Table.FTVal (Pipit.Prim.HasStream.shallow bool))))
+  op_Equality
+
+unfold let __xprim_mm_v2b_opt_eq_int_40 : Pipit.Prim.Shallow.prim =
+  Pipit.Prim.Shallow.Mkprim (Some "Prims.op_Equality")
+  (Pipit.Prim.Table.FTFun (Pipit.Prim.HasStream.shallow mode)
+      (Pipit.Prim.Table.FTFun (Pipit.Prim.HasStream.shallow mode)
+          (Pipit.Prim.Table.FTVal (Pipit.Prim.HasStream.shallow bool))))
+  op_Equality
+
+unfold let __xprim_mm_v2b_opt_eq_int_39 : Pipit.Prim.Shallow.prim =
+  Pipit.Prim.Shallow.Mkprim (Some "Prims.op_BarBar")
+  (Pipit.Prim.Table.FTFun (Pipit.Prim.HasStream.shallow bool)
+      (Pipit.Prim.Table.FTFun (Pipit.Prim.HasStream.shallow bool)
+          (Pipit.Prim.Table.FTVal (Pipit.Prim.HasStream.shallow bool))))
+  op_BarBar
+
+unfold let __xprim_mm_v2b_opt_eq_int_38 : Pipit.Prim.Shallow.prim =
+  Pipit.Prim.Shallow.Mkprim (Some "PipitRuntime.Prim.p'select")
+  (Pipit.Prim.Table.FTFun (Pipit.Prim.HasStream.shallow bool)
+      (Pipit.Prim.Table.FTFun (Pipit.Prim.HasStream.shallow master_mode)
+          (Pipit.Prim.Table.FTFun (Pipit.Prim.HasStream.shallow master_mode)
+              (Pipit.Prim.Table.FTVal (Pipit.Prim.HasStream.shallow master_mode)))))
+  PipitRuntime.Prim.p'select
+
+let mm_v2b_opt_eq_int_core (cfg: config_int) : Pipit.Exp.Base.exp Pipit.Prim.Shallow.table
+  [Pipit.Prim.HasStream.shallow (option master_index_int);
+   Pipit.Prim.HasStream.shallow error_severity;
+   Pipit.Prim.HasStream.shallow mode]
+  (Pipit.Prim.HasStream.shallow master_mode) =
+  (fun master_enable ->
+      (fun master_idx ->
+          Pipit.Exp.Base.XLet (Pipit.Prim.HasStream.shallow master_mode)
+            (Pipit.Exp.Base.XMu
+              (Pipit.Exp.Base.XLet (Pipit.Prim.HasStream.shallow master_mode)
+                  (Pipit.Exp.Base.XFby Master_Off (Pipit.Exp.Base.XBase (Pipit.Exp.Base.XBVar 0)))
+                  (Pipit.Exp.Base.XApps
+                    (Pipit.Exp.Base.XApp
+                        (Pipit.Exp.Base.XApp
+                            (Pipit.Exp.Base.XApp
+                                (Pipit.Exp.Base.XPrim
+                                  __xprim_mm_v2b_opt_eq_int_38)
+                                (Pipit.Exp.Base.XApps
+                                  (Pipit.Exp.Base.XApp
+                                      (Pipit.Exp.Base.XApp
+                                          (Pipit.Exp.Base.XPrim
+                                            __xprim_mm_v2b_opt_eq_int_39
+                                          )
+                                          (Pipit.Exp.Base.XApps
+                                            (Pipit.Exp.Base.XApp
+                                                (Pipit.Exp.Base.XApp
+                                                    (Pipit.Exp.Base.XPrim
+                                                      __xprim_mm_v2b_opt_eq_int_40
+                                                    )
+                                                    (Pipit.Exp.Base.XBase (Pipit.Exp.Base.XBVar 4)))
+                                                (Pipit.Exp.Base.XBase
+                                                  (Pipit.Exp.Base.XVal Mode_Configure)))))
+                                      (Pipit.Exp.Base.XApps
+                                        (Pipit.Exp.Base.XApp
+                                            (Pipit.Exp.Base.XApp
+                                                (Pipit.Exp.Base.XPrim
+                                                  __xprim_mm_v2b_opt_eq_int_41
+                                                ) (Pipit.Exp.Base.XBase (Pipit.Exp.Base.XBVar 3)))
+                                            (Pipit.Exp.Base.XBase (Pipit.Exp.Base.XVal S3_Severe))))
+                                  ))) (Pipit.Exp.Base.XBase (Pipit.Exp.Base.XVal Master_Off)))
+                        (Pipit.Exp.Base.XApps
+                          (Pipit.Exp.Base.XApp
+                              (Pipit.Exp.Base.XApp
+                                  (Pipit.Exp.Base.XApp
+                                      (Pipit.Exp.Base.XPrim
+                                        __xprim_mm_v2b_opt_eq_int_38
+                                      )
+                                      (Pipit.Exp.Base.XApps
+                                        (Pipit.Exp.Base.XApp
+                                            (Pipit.Exp.Base.XApp
+                                                (Pipit.Exp.Base.XPrim
+                                                  __xprim_mm_v2b_opt_eq_int_42
+                                                ) (Pipit.Exp.Base.XBase (Pipit.Exp.Base.XBVar 0)))
+                                            (Pipit.Exp.Base.XBase (Pipit.Exp.Base.XVal Master_Off)))
+                                      ))
+                                  (Pipit.Exp.Base.XApps
+                                    (Pipit.Exp.Base.XApp
+                                        (Pipit.Exp.Base.XApp
+                                            (Pipit.Exp.Base.XApp
+                                                (Pipit.Exp.Base.XPrim
+                                                  __xprim_mm_v2b_opt_eq_int_38
+                                                )
+                                                (Pipit.Exp.Base.XApps
+                                                  (Pipit.Exp.Base.XApp
+                                                      (Pipit.Exp.Base.XApp
+                                                          (Pipit.Exp.Base.XPrim
+                                                            __xprim_mm_v2b_opt_eq_int_43
+                                                          )
+                                                          (Pipit.Exp.Base.XApps
+                                                            (Pipit.Exp.Base.XApp
+                                                                (Pipit.Exp.Base.XPrim
+                                                                  __xprim_mm_v2b_opt_eq_int_44
+                                                                )
+                                                                (Pipit.Exp.Base.XBase
+                                                                  (Pipit.Exp.Base.XBVar 2)))))
+                                                      (Pipit.Exp.Base.XBase
+                                                        (Pipit.Exp.Base.XVal
+                                                          (op_Negation master_enable))))))
+                                            (Pipit.Exp.Base.XBase (Pipit.Exp.Base.XVal Follower)))
+                                        (Pipit.Exp.Base.XApps
+                                          (Pipit.Exp.Base.XApp
+                                              (Pipit.Exp.Base.XApp
+                                                  (Pipit.Exp.Base.XApp
+                                                      (Pipit.Exp.Base.XPrim
+                                                        __xprim_mm_v2b_opt_eq_int_38
+                                                      )
+                                                      (Pipit.Exp.Base.XApps
+                                                        (Pipit.Exp.Base.XApp
+                                                            (Pipit.Exp.Base.XApp
+                                                                (Pipit.Exp.Base.XPrim
+                                                                  __xprim_mm_v2b_opt_eq_int_43
+                                                                )
+                                                                (Pipit.Exp.Base.XApps
+                                                                  (Pipit.Exp.Base.XApp
+                                                                      (Pipit.Exp.Base.XApp
+                                                                          (Pipit.Exp.Base.XPrim
+                                                                            __xprim_mm_v2b_opt_eq_int_43
+                                                                          )
+                                                                          (Pipit.Exp.Base.XApps
+                                                                            (Pipit.Exp.Base.XApp
+                                                                                (Pipit.Exp.Base.XPrim
+                                                                                  __xprim_mm_v2b_opt_eq_int_44
+                                                                                )
+                                                                                (Pipit.Exp.Base.XBase
+                                                                                  (Pipit.Exp.Base.XBVar
+                                                                                    2)))))
+                                                                      (Pipit.Exp.Base.XBase
+                                                                        (Pipit.Exp.Base.XVal
+                                                                          master_enable)))))
+                                                            (Pipit.Exp.Base.XApps
+                                                              (Pipit.Exp.Base.XApp
+                                                                  (Pipit.Exp.Base.XApp
+                                                                      (Pipit.Exp.Base.XPrim
+                                                                        __xprim_mm_v2b_opt_eq_int_45
+                                                                      )
+                                                                      (Pipit.Exp.Base.XBase
+                                                                        (Pipit.Exp.Base.XBVar 3)))
+                                                                  (Pipit.Exp.Base.XBase
+                                                                    (Pipit.Exp.Base.XVal S2_Error)))
+                                                            ))))
+                                                  (Pipit.Exp.Base.XApps
+                                                    (Pipit.Exp.Base.XApp
+                                                        (Pipit.Exp.Base.XApp
+                                                            (Pipit.Exp.Base.XApp
+                                                                (Pipit.Exp.Base.XPrim
+                                                                  __xprim_mm_v2b_opt_eq_int_38
+                                                                )
+                                                                (Pipit.Exp.Base.XApps
+                                                                  (Pipit.Exp.Base.XApp
+                                                                      (Pipit.Exp.Base.XApp
+                                                                          (Pipit.Exp.Base.XPrim
+                                                                            __xprim_mm_v2b_opt_eq_int_46
+                                                                          )
+                                                                          (Pipit.Exp.Base.XBase
+                                                                            (Pipit.Exp.Base.XBVar 2)
+                                                                          ))
+                                                                      (Pipit.Exp.Base.XBase
+                                                                        (Pipit.Exp.Base.XVal
+                                                                          (Some master_idx))))))
+                                                            (Pipit.Exp.Base.XBase
+                                                              (Pipit.Exp.Base.XVal Current_Master)))
+                                                        (Pipit.Exp.Base.XBase
+                                                          (Pipit.Exp.Base.XVal Backup_Master)))))
+                                              (Pipit.Exp.Base.XBase (Pipit.Exp.Base.XVal Master_Off)
+                                              )))))) (Pipit.Exp.Base.XBase (Pipit.Exp.Base.XBVar 0))
+                          ))))))
+            (Pipit.Exp.Base.XBase (Pipit.Exp.Base.XBVar 0))) cfg.master_idx) cfg.master_enable
